## Negation
$$
\lnot(P \Rightarrow Q) = P \land \lnot Q
$$
## Contraposition
- we know that $$
P \Rightarrow Q = Q \lor \neg P
$$
- this can be rewritten as 
$$
\neg P \lor Q
$$
- or even
$$
\neg P \lor \neg(\neg Q)
$$
- therefore
$$
P \Rightarrow Q = \neg Q \Rightarrow \neg P
$$
## Quantifiers
### Universal Quantifier
- we write for all $x, P(x)$ or $\forall x, P(x)$ where $P(x)$ is a proposition involving $x$
### Existential Quantifier
- we write there exists $x$ such that $P(x)$ or $\exists x, P(x)$ where $P(x)$ is a proposition involving  $x$
- prove by:
	- exhibiting an example
	- use a theorem that guarantees existence of an example